More assembly code clean up (dissassemble is broken)

12AssemblyCode/AssemblyCode.thy
@@ -16,16 +16,18 @@ environment heap, value stack, and callstack, and one as an accumulator. It also
 register for the code-pointer, and an infinite natural-indexed memory.\<close>
 
 text \<open>For this stage, in order to ease the already quite-involved conversion, we imbue the processor 
-with a little more structure. We tag each memory cell and the accumulator register with a memory 
-segment, to say what kind of pointer lives in it. (\<open>Acc\<close> stands for non-pointers.) We also keep our 
-four memory segments separate in the memory map; this leaves us with an extra segment for \<open>Acc\<close> but
-it will remain unused and we will arrange to allocate no space for it in the final memory layout.\<close>
+with a little more structure. We tag each memory cell and register with a memory segment, to say 
+what kind of pointer lives in it. (\<open>Acc\<close> stands for non-pointers; the tag for all registers except 
+\<open>Acc\<close> will be the same as the register itself, but the uniformity of tagging all of them simplifies 
+the representation and is helpful to later proofs.) We also keep our four memory segments separate 
+in the memory map; this leaves us with an extra segment for \<open>Acc\<close> but it will remain unused and we 
+will arrange to allocate no space for it in the final memory layout.\<close>
 
 datatype memseg = Hp | Env | Vals | Stk | Acc
 
-datatype assm_state = S\<^sub>a "memseg \<Rightarrow> nat \<Rightarrow> memseg \<times> nat" "memseg \<Rightarrow> nat" memseg nat
+datatype assm_state = S\<^sub>a "memseg \<times> nat \<Rightarrow> memseg \<times> nat" "memseg \<Rightarrow> memseg \<times> nat" nat
 
-text \<open>We have a small, RISC-like (not to say minimalistic) set of operations on the processor. We 
+text \<open>We have a small, RISC-like (not to say minimalistic) set of operations for the processor. We 
 can do simple arithmetic on the registers; we can move values between registers, and load and store 
 into memory; and we can jump, to a static address or indirectly to an address in a register. We will
 not need all of even this small set of functionality (we never add or subtract a non-constant, or 
@@ -34,189 +36,84 @@ expansion of the source language.\<close>
 
 text \<open>In our assembler, we allow ourselves some liberties with the opcodes. The operate-on-register/
 operate-on-constant opcodes are collapsed into a single assembly operation; and the move/load/store 
-operations are likewise reduced to a single \<open>AMov\<close> operation with a number of addressing modes.\<close>
+operations are likewise reduced to a single \<open>AMov\<close> operation with a number of addressing modes. We 
+do not syntactically rule out every invalid combination: \<open>AMov (Con 0) (Con 2)\<close> is permitted, for 
+instance, even though you obviously cannot assign to the constant 0. Invalid operations, instead,
+have no associated transition. There are a few less obvious invalid operations: for instance, in 
+keeping with our desire to make a RISC-style processor, you cannot directly add the contents of 
+memory to a register; it has to be explicitly loaded into another register with an \<open>AMov\<close> operation 
+first.\<close>
 
-datatype addr_mode = Reg memseg | Con nat
-
-datatype move_src = Reg memseg | Con nat | Mem memseg
+datatype addr_mode = Reg memseg | Con nat | Mem memseg
 
 datatype assm = 
-  APut memseg move_src
+  AMov addr_mode addr_mode
   | ASub memseg nat
   | AAdd memseg nat
   | AJmp
 
-fun mem_upd :: "(memseg \<Rightarrow> nat \<Rightarrow> memseg \<times> nat) \<Rightarrow> memseg \<Rightarrow> nat \<Rightarrow> memseg \<times> nat \<Rightarrow> 
-    memseg \<Rightarrow> nat \<Rightarrow> memseg \<times> nat" where
-  "mem_upd mem m mp k m' x = (if m = m' \<and> mp = x then k else mem m' x)"
-
-inductive evala :: "assm list \<Rightarrow> assm_state \<Rightarrow> assm_state \<Rightarrow> bool" (infix "\<tturnstile> _ \<leadsto>\<^sub>a" 50) where
-  eva_movr [simp]: "lookup cd pc = Some (APut Acc (Reg r)) \<Longrightarrow> r \<noteq> Acc \<Longrightarrow>
-    cd \<tturnstile> S\<^sub>a mem ps act (Suc pc) \<leadsto>\<^sub>a S\<^sub>a mem (ps(Acc := ps r)) r pc"
-| eva_mova [simp]: "lookup cd pc = Some (APut Acc (Reg Acc)) \<Longrightarrow> 
-    cd \<tturnstile> S\<^sub>a mem ps act (Suc pc) \<leadsto>\<^sub>a S\<^sub>a mem ps act pc"
-| eva_movk [simp]: "lookup cd pc = Some (APut Acc (Con k)) \<Longrightarrow> 
-    cd \<tturnstile> S\<^sub>a mem ps act (Suc pc) \<leadsto>\<^sub>a S\<^sub>a mem (ps(Acc := k)) Acc pc"
-| eva_lod [simp]: "lookup cd pc = Some (APut Acc (Mem r')) \<Longrightarrow> mem r' (ps r') = (t, b) \<Longrightarrow> r' \<noteq> Acc \<Longrightarrow>
-    cd \<tturnstile> S\<^sub>a mem ps act (Suc pc) \<leadsto>\<^sub>a S\<^sub>a mem (ps(Acc := b)) t pc"
-| eva_loda [simp]: "lookup cd pc = Some (APut Acc (Mem Acc)) \<Longrightarrow> mem act (ps Acc) = (t, b) \<Longrightarrow> act \<noteq> Acc \<Longrightarrow>
-    cd \<tturnstile> S\<^sub>a mem ps act (Suc pc) \<leadsto>\<^sub>a S\<^sub>a mem (ps(Acc := b)) t pc"
-| eva_putr [simp]: "lookup cd pc = Some (APut r (Reg r')) \<Longrightarrow> r \<noteq> Acc \<Longrightarrow> r' \<noteq> Acc \<Longrightarrow>
-    cd \<tturnstile> S\<^sub>a mem ps act (Suc pc) \<leadsto>\<^sub>a S\<^sub>a (mem_upd mem r (ps r) (r', ps r')) ps act pc"
-| eva_puta [simp]: "lookup cd pc = Some (APut r (Reg Acc)) \<Longrightarrow> r \<noteq> Acc \<Longrightarrow>
-    cd \<tturnstile> S\<^sub>a mem ps act (Suc pc) \<leadsto>\<^sub>a S\<^sub>a (mem_upd mem r (ps r) (act, ps Acc)) ps act pc"
-| eva_putk [simp]: "lookup cd pc = Some (APut r (Con k)) \<Longrightarrow> r \<noteq> Acc \<Longrightarrow>
-    cd \<tturnstile> S\<^sub>a mem ps act (Suc pc) \<leadsto>\<^sub>a S\<^sub>a (mem_upd mem r (ps r) (Acc, k)) ps act pc"
-| eva_get [simp]: "lookup cd pc = Some (APut r (Mem r')) \<Longrightarrow> mem r' (ps r') = (r, b) \<Longrightarrow> 
-      r' \<noteq> Acc \<Longrightarrow> r \<noteq> Acc \<Longrightarrow>
-    cd \<tturnstile> S\<^sub>a mem ps act (Suc pc) \<leadsto>\<^sub>a S\<^sub>a mem (ps(r := b)) act pc"
-| eva_geta [simp]: "lookup cd pc = Some (APut r (Mem Acc)) \<Longrightarrow> mem act (ps Acc) = (r, b) \<Longrightarrow> 
-      r \<noteq> Acc \<Longrightarrow> act \<noteq> Acc \<Longrightarrow>
-    cd \<tturnstile> S\<^sub>a mem ps act (Suc pc) \<leadsto>\<^sub>a S\<^sub>a mem (ps(r := b)) act pc"
-| eva_suba [simp]: "lookup cd pc = Some (ASub Acc k) \<Longrightarrow> ps Acc \<ge> k \<Longrightarrow> act \<noteq> Acc \<Longrightarrow>
-    cd \<tturnstile> S\<^sub>a mem ps act (Suc pc) \<leadsto>\<^sub>a S\<^sub>a mem (ps(Acc := ps Acc - k)) act pc"
-| eva_sub [simp]: "lookup cd pc = Some (ASub r k) \<Longrightarrow> ps r \<ge> k \<Longrightarrow> r \<noteq> Acc \<Longrightarrow>
-    cd \<tturnstile> S\<^sub>a mem ps act (Suc pc) \<leadsto>\<^sub>a S\<^sub>a mem (ps(r := ps r - k)) act pc"
-| eva_add [simp]: "lookup cd pc = Some (AAdd r k) \<Longrightarrow> r \<noteq> Acc \<Longrightarrow>
-    cd \<tturnstile> S\<^sub>a mem ps act (Suc pc) \<leadsto>\<^sub>a S\<^sub>a mem (ps(r := ps r + k)) act pc"
-| eva_adda [simp]: "lookup cd pc = Some (AAdd Acc k) \<Longrightarrow> act \<noteq> Acc \<Longrightarrow>
-    cd \<tturnstile> S\<^sub>a mem ps act (Suc pc) \<leadsto>\<^sub>a S\<^sub>a mem (ps(Acc := ps Acc + k)) act pc"
-| eva_jmp [simp]: "lookup cd pc = Some AJmp \<Longrightarrow> 
-    cd \<tturnstile> S\<^sub>a mem ps Acc (Suc pc) \<leadsto>\<^sub>a S\<^sub>a mem (ps(Acc := 0)) Acc (ps Acc)"
-
 abbreviation reg_merge :: "memseg \<Rightarrow> memseg \<Rightarrow> memseg" where
   "reg_merge a b \<equiv> (if a = Acc then b else a)"
 
-fun assm_step :: "(memseg \<Rightarrow> nat \<Rightarrow> memseg \<times> nat) \<Rightarrow> (memseg \<Rightarrow> nat) \<Rightarrow> memseg \<Rightarrow> nat \<Rightarrow> 
+fun assm_step :: "(memseg \<times> nat \<Rightarrow> memseg \<times> nat) \<Rightarrow> (memseg \<Rightarrow> memseg \<times> nat) \<Rightarrow> nat \<Rightarrow> 
     assm \<rightharpoonup> assm_state" where
-  "assm_step mem ps act pc (APut Acc (Reg r')) = 
-    Some (S\<^sub>a mem (ps(Acc := ps r')) (reg_merge r' act) pc)"
-| "assm_step mem ps act pc (APut Acc (Con k)) = 
-    Some (S\<^sub>a mem (ps(Acc := k)) Acc pc)"
-| "assm_step mem ps act pc (APut Acc (Mem r')) = (case mem (reg_merge r' act) (ps r') of
-     (t, b) \<Rightarrow> if r' \<noteq> Acc \<or> act \<noteq> Acc then Some (S\<^sub>a mem (ps(Acc := b)) t pc) else None)"
-| "assm_step mem ps act pc (APut r (Reg r')) = 
-    Some (S\<^sub>a (mem_upd mem r (ps r) (reg_merge r' act, ps r')) ps act pc)"
-| "assm_step mem ps act pc (APut r (Con k)) = 
-    Some (S\<^sub>a (mem_upd mem r (ps r) (Acc, k)) ps act pc)"
-| "assm_step mem ps act pc (APut r (Mem r')) = (case mem (reg_merge r' act) (ps r') of
-     (t, b) \<Rightarrow> if t = r \<and> (r' \<noteq> Acc \<or> act \<noteq> Acc) then Some (S\<^sub>a mem (ps(r := b)) act pc) else None)"
-| "assm_step mem ps act pc (ASub r k) = 
-    (if ps r < k \<or> (r = Acc \<and> act = Acc) then None 
-     else Some (S\<^sub>a mem (ps(r := ps r - k)) act pc))"
-| "assm_step mem ps act pc (AAdd r k) = 
-    (if r = Acc \<and> act = Acc then None 
-     else Some (S\<^sub>a mem (ps(r := ps r + k)) act pc))"
-| "assm_step mem ps act pc AJmp = 
-    (if act = Acc then Some (S\<^sub>a mem (ps(Acc := 0)) Acc (ps Acc)) else None)"
+  "assm_step mem ps pc (AMov (Reg r) (Reg r')) = Some (S\<^sub>a mem (ps(r := ps r')) pc)"
+| "assm_step mem ps pc (AMov (Reg r) (Con k)) = Some (S\<^sub>a mem (ps(r := (Acc, k))) pc)"
+| "assm_step mem ps pc (AMov (Reg r) (Mem r')) = Some (S\<^sub>a mem (ps(r := mem (ps r'))) pc)"
+| "assm_step mem ps pc (AMov (Con k) x) = None"
+| "assm_step mem ps pc (AMov (Mem r) (Reg r')) = Some (S\<^sub>a (mem(ps r := ps r')) ps pc)"
+| "assm_step mem ps pc (AMov (Mem r) (Con k)) = Some (S\<^sub>a (mem(ps r := (Acc, k))) ps pc)"
+| "assm_step mem ps pc (AMov (Mem r) (Mem r')) = None"
+| "assm_step mem ps pc (ASub r k) = (case ps r of
+    (t, v) \<Rightarrow> if v < k then None else Some (S\<^sub>a mem (ps(r := (t, v - k))) pc))"
+| "assm_step mem ps pc (AAdd r k) = (case ps r of
+    (t, v) \<Rightarrow> Some (S\<^sub>a mem (ps(r := (t, v + k))) pc))"
+| "assm_step mem ps pc AJmp = (case ps Acc of
+    (t, v) \<Rightarrow> if t = Acc then Some (S\<^sub>a mem (ps(Acc := (Acc, 0))) v) else None)"
 
-fun alg_evala :: "assm list \<Rightarrow> assm_state \<rightharpoonup> assm_state" (infix "\<tturnstile>\<^sub>a" 50) where
-  "cd \<tturnstile>\<^sub>a S\<^sub>a mem ps act pc = (case pc of
+primrec eval\<^sub>a :: "assm list \<Rightarrow> assm_state \<rightharpoonup> assm_state" where
+  "eval\<^sub>a cd (S\<^sub>a mem ps pc) = (case pc of
       0 \<Rightarrow> None
-    | Suc pc \<Rightarrow> Option.bind (lookup cd pc) (assm_step mem ps act pc))"
+    | Suc pc' \<Rightarrow> Option.bind (lookup cd pc') (assm_step mem ps pc'))"
 
-primrec iter_evala :: "assm list \<Rightarrow> nat \<Rightarrow> assm_state \<rightharpoonup> assm_state" where
-  "iter_evala cd 0 \<Sigma> = Some \<Sigma>"
-| "iter_evala cd (Suc x) \<Sigma> = Option.bind (cd \<tturnstile>\<^sub>a \<Sigma>) (iter_evala cd x)"
+primrec iter_eval\<^sub>a :: "assm list \<Rightarrow> nat \<Rightarrow> assm_state \<rightharpoonup> assm_state" where
+  "iter_eval\<^sub>a cd 0 \<Sigma> = Some \<Sigma>"
+| "iter_eval\<^sub>a cd (Suc x) \<Sigma> = Option.bind (eval\<^sub>a cd \<Sigma>) (iter_eval\<^sub>a cd x)"
 
-lemma [simp]: "mem_upd (case_memseg h e vs sh a) Hp x y = case_memseg (h(x := y)) e vs sh a"
-proof (rule, rule)
-  fix m n
-  show "mem_upd (case_memseg h e vs sh a) Hp x y m n = case_memseg (h(x := y)) e vs sh a m n"
-    by (induction m) (simp_all split: memseg.splits)
-qed
+abbreviation some_eval\<^sub>a :: "assm list \<Rightarrow> assm_state \<Rightarrow> assm_state \<Rightarrow> bool" (infix "\<tturnstile> _ \<leadsto>\<^sub>a" 50) where
+  "cd \<tturnstile> \<Sigma> \<leadsto>\<^sub>a \<Sigma>' \<equiv> (eval\<^sub>a cd \<Sigma> = Some \<Sigma>')"
 
-lemma [simp]: "mem_upd (case_memseg h e vs sh a) Env x y = case_memseg h (e(x := y)) vs sh a"
-proof (rule, rule)
-  fix m n
-  show "mem_upd (case_memseg h e vs sh a) Env x y m n = case_memseg h (e(x := y)) vs sh a m n"
-    by (induction m) (simp_all split: memseg.splits)
-qed
-
-lemma [simp]: "mem_upd (case_memseg h e vs sh a) Vals x y = case_memseg h e (vs(x := y)) sh a"
-proof (rule, rule)
-  fix m n
-  show "mem_upd (case_memseg h e vs sh a) Vals x y m n = case_memseg h e (vs(x := y)) sh a m n"
-    by (induction m) (simp_all split: memseg.splits)
-qed
-
-lemma [simp]: "mem_upd (case_memseg h e vs sh a) Stk x y = case_memseg h e vs (sh(x := y)) a"
-proof (rule, rule)
-  fix m n
-  show "mem_upd (case_memseg h e vs sh a) Stk x y m n = case_memseg h e vs (sh(x := y)) a m n"
-    by (induction m) (simp_all split: memseg.splits)
-qed
-
-lemma iter_evala_combine [simp]: "iter_evala cd n \<Sigma> = Some \<Sigma>' \<Longrightarrow> 
-  iter_evala cd m \<Sigma>' = Some \<Sigma>'' \<Longrightarrow> iter_evala cd (n + m) \<Sigma> = Some \<Sigma>''"
+lemma iter_evala_combine [simp]: "iter_eval\<^sub>a cd n \<Sigma> = Some \<Sigma>' \<Longrightarrow> 
+  iter_eval\<^sub>a cd m \<Sigma>' = Some \<Sigma>'' \<Longrightarrow> iter_eval\<^sub>a cd (n + m) \<Sigma> = Some \<Sigma>''"
 proof (induction n arbitrary: \<Sigma>)
   case (Suc n)
-  then show ?case by (cases "cd \<tturnstile>\<^sub>a \<Sigma>") simp_all
+  then show ?case by (cases "eval\<^sub>a cd \<Sigma>") simp_all
 qed simp_all
 
-lemma assm_step_equiv: "(Option.bind (lookup cd pc) (assm_step mem ps act pc) = Some \<Sigma>) \<Longrightarrow>
-  (cd \<tturnstile> S\<^sub>a mem ps act (Suc pc) \<leadsto>\<^sub>a \<Sigma>)"
-proof (cases "lookup cd pc")
-  case (Some op)
-  moreover assume "Option.bind (lookup cd pc) (assm_step mem ps act pc) = Some \<Sigma>"
-  ultimately show ?thesis 
-  proof (induction mem ps act pc op rule: assm_step.induct)
-    case (7 mem ps act pc r k)
-    then show ?case by (cases r) (auto split: if_splits)
-  next
-    case (8 mem ps act pc r k)
-    then show ?case by (cases r) (auto split: if_splits)
-  qed (auto split: if_splits prod.splits option.splits)
-qed simp_all
-
-lemma alg_evala_equiv: "(cd \<tturnstile> \<Sigma> \<leadsto>\<^sub>a \<Sigma>') = (cd \<tturnstile>\<^sub>a \<Sigma> = Some \<Sigma>')"
-proof
-  show "cd \<tturnstile>\<^sub>a \<Sigma> = Some \<Sigma>' \<Longrightarrow> cd \<tturnstile> \<Sigma> \<leadsto>\<^sub>a \<Sigma>'"
-    by (induction \<Sigma>) (auto simp add: assm_step_equiv split: nat.splits)
-  show "cd \<tturnstile> \<Sigma> \<leadsto>\<^sub>a \<Sigma>' \<Longrightarrow> cd \<tturnstile>\<^sub>a \<Sigma> = Some \<Sigma>'" 
-  proof (induction cd \<Sigma> \<Sigma>' rule: evala.induct)
-    case (eva_putr cd pc r r' mem ps act)
-    thus ?case by (induction r) simp_all
-  next
-    case (eva_puta cd pc r mem ps act)
-    thus ?case by (induction r) simp_all
-  next
-    case (eva_putk cd pc r k mem ps act)
-    thus ?case by (induction r) simp_all
-  next
-    case (eva_get cd pc r r' mem ps b act)
-    thus ?case by (induction r) simp_all
-  next
-    case (eva_geta cd pc r mem act ps b)
-    thus ?case by (induction r) simp_all
-  qed simp_all
-qed
-
-lemma iter_evala_equiv: "iter (\<tturnstile> cd \<leadsto>\<^sub>a) \<Sigma> \<Sigma>' = (\<exists>n. iter_evala cd n \<Sigma> = Some \<Sigma>')"
-proof
-  assume "\<exists>n. iter_evala cd n \<Sigma> = Some \<Sigma>'"
-  then obtain n where "iter_evala cd n \<Sigma> = Some \<Sigma>'" by fastforce
-  thus "iter (\<tturnstile> cd \<leadsto>\<^sub>a) \<Sigma> \<Sigma>'" 
-  proof (induction n arbitrary: \<Sigma>)
-    case (Suc n)
-    thus ?case by (cases "cd \<tturnstile>\<^sub>a \<Sigma>") (simp_all add: alg_evala_equiv)
-  qed simp_all
-next
-  show "iter (\<tturnstile> cd \<leadsto>\<^sub>a) \<Sigma> \<Sigma>' \<Longrightarrow> \<exists>n. iter_evala cd n \<Sigma> = Some \<Sigma>'" 
+lemma iter_evala_equiv [simp]: "iter (\<tturnstile> cd \<leadsto>\<^sub>a) \<Sigma> \<Sigma>' = (\<exists>n. iter_eval\<^sub>a cd n \<Sigma> = Some \<Sigma>')"
+proof 
+  show "iter (\<tturnstile> cd \<leadsto>\<^sub>a) \<Sigma> \<Sigma>' \<Longrightarrow> \<exists>n. iter_eval\<^sub>a cd n \<Sigma> = Some \<Sigma>'" 
   proof (induction \<Sigma> \<Sigma>' rule: iter.induct)
     case (iter_refl \<Sigma>)
-    have "iter_evala cd 0 \<Sigma> = Some \<Sigma>" by simp
+    have "iter_eval\<^sub>a cd 0 \<Sigma> = Some \<Sigma>" by simp
     thus ?case by blast
   next
     case (iter_step \<Sigma> \<Sigma>' \<Sigma>'')
-    then obtain n where "iter_evala cd n \<Sigma>' = Some \<Sigma>''" by fastforce
-    moreover from iter_step have "cd \<tturnstile>\<^sub>a \<Sigma> = Some \<Sigma>'" by (simp add: alg_evala_equiv)
-    ultimately have "iter_evala cd (Suc n) \<Sigma> = Some \<Sigma>''" by simp
+    moreover then obtain n where "iter_eval\<^sub>a cd n \<Sigma>' = Some \<Sigma>''" by blast
+    ultimately have "iter_eval\<^sub>a cd (Suc n) \<Sigma> = Some \<Sigma>''" by simp
     thus ?case by blast
   qed
+next
+  assume "\<exists>n. iter_eval\<^sub>a cd n \<Sigma> = Some \<Sigma>'"
+  then obtain n where "iter_eval\<^sub>a cd n \<Sigma> = Some \<Sigma>'" by blast
+  thus "iter (\<tturnstile> cd \<leadsto>\<^sub>a) \<Sigma> \<Sigma>'" 
+  proof (induction n arbitrary: \<Sigma>)
+    case (Suc n)
+    thus ?case by (cases "eval\<^sub>a cd \<Sigma>") simp_all
+  qed simp_all
 qed
 
 theorem determinisma: "cd \<tturnstile> \<Sigma> \<leadsto>\<^sub>a \<Sigma>' \<Longrightarrow> cd \<tturnstile> \<Sigma> \<leadsto>\<^sub>a \<Sigma>'' \<Longrightarrow> \<Sigma>' = \<Sigma>''"
-  by (simp add: alg_evala_equiv)
+  by simp
 
 end
