00Utils/Utils.thy
@@ -103,7 +103,10 @@ lemma snd_pair [simp]: "(a, b) = f x \<Longrightarrow> snd (f x) = b"
 lemma plus_zero [simp]: "(+) (0::nat) = id"
   by auto
 
-lemma [simp]: "odd (x::nat) \<Longrightarrow> 0 < x"
-  by (cases x) simp_all
+lemma suc_even [simp]: "Suc (Suc 0) dvd Suc x \<Longrightarrow> odd x"
+  by presburger
+
+lemma even_down [simp]: "Suc (Suc 0) dvd Suc (Suc x) = (Suc (Suc 0) dvd x)"
+  by presburger
 
 end
